@prefix scribejs: <https://w3c.github.io/scribjes/vocab/>.
@prefix rdfs:     <http://www.w3.org/2000/01/rdf-schema#>.
@prefix owl:      <http://www.w3.org/2002/07/owl#>.
@prefix rdf:      <http://www.w3.org/1999/02/22-rdf-syntax-ns#>.
@prefix schema:   <https://schema.org>.
@prefix xsd:      <http://www.w3.org/2001/XMLSchema#> .
@prefix sh:       <http://www.w3.org/ns/shacl#> .
@base <https://w3c.github.io/scribjes/vocab/>



:Resolution a rdfs:Class ;
    rdfs:comment "a type identifying an object describing a resolution of a meeting, and recorded in the minutes as such"
.

:resolution a rdf:Property ;
    rdfs:domain schema:CreativeWork ;
    rdfs:range scribejs:Resolution ;
    rdfs:comment "a property referring to a resolution object"
.

:resolution_number a rdf:Property ;
    rdfs:domain scribejs:Resolution ;
    rdfs:range xsd:integer ;
    rdfs:comment "a property referring to the number identifier of a resolution object"
.

:resolution_text a rdf:Property ;
    rdfs:domain scribejs:Resolution ;
    rdfs:range xsd:string ;
    rdfs:comment "a property referring to the text of the resolution "
.

:irc a rdf:Property ;
    rdfs:domain schema:CreativeWork ;
    rdfs:range xsd:string ;
    rdfs:comment "a property referring to the irc channel used for the minutes"
.


:CreativeWorkShape a sh:NodeShape ;
    sh:targetClass schema:CreativeWork ;
    sh:property
        [
            sh:path :resolution ;
            sh:nodeKind sh:BlankNodeOrIRI ;
            sh:class :Resolution
        ],[
            sh:path :irc ;
            sh:nodeKind sh:Literal ;
            sh:maxCount 1
        ];
.

:ResolutionShape a sh:NodeShape ;
    sh:targetClass :Resolution ;
    sh:property
        [
            sh:path :resolution_number ;
            sh:datatype xsd:integer ;
            sh:maxCount 1
        ],[
            sh:path :resolution_text ;
            sh:datatype xsd:string ;
            sh:maxCount 1
        ];
    sh:closed true ;
.
